Read write ideal (#28)
* Find keys and add to heap upon receiving message, or decrypting message
* issue-less change since it's so fundamental to the real world model

KeyManagement/IdealWorld.v
@@ -1,214 +1,97 @@
 From Coq Require Import String.
 From Coq Require Import Bool.Sumbool.
 Require Import Frap.
-Require Import Common.
 Set Implicit Arguments.
+
+Definition user_id := var.
 
 Definition channel_id := nat.
 
-(*
- *
- * Description of channels which allow users to send messages with certain security properties.
- *
- *)
-(* High level definition of security can be defined as a subset of CIA. *)
-Record security_properties := construct_properties
-  { confidentiality : bool ;
-    authenticity : bool ;
-    integrity : bool ; }.
+Record permission := construct_permission
+  { read : bool ;
+    write : bool }.
 
-(* Two kinds of channels follow from the mere presence of a user in universe since users are defined as a 
-   named entity (real world analog: the owner of a public key). Consider each case from A's perspective:
-   - Default channels
-     - two owners with equal privileges 
-     - always CIA
-     - users may send 
-     - real world analog is using B's public key to encrypt a message signed by A's private key
-   - Broadcast Channels
-     - have single owner
-     - either confidential to owner or authentic (integrity follows) to owner
-     - "real world" analog is signing with A's public key or encrypting with B's public key
+Definition permissions := fmap channel_id permission.
 
-   Users themselves can create symmetric channels with a given set of properties
-   - some restrictions since an authentic symmetric channel is impossible with more than 2 users
-   - "real world" analog is using symmetric HMAC and/or symmetric encryption with shared key
-*)
-Inductive channel_type :=
-| Default : user_id -> user_id -> channel_type
-| Broadcast : user_id -> channel_type
-| Symmetric : channel_type.
+Definition creator_permission := construct_permission true true.
 
+Inductive message : Type -> Type :=
+| Permission (id : channel_id) (p : permission) : message (channel_id * permission)
+| Content {A : Type} (m : A) : message A
+| MsgPair {A B : Type} (m1 : message A) (m2 : message B) : message (A * B).
 
 (* Exisistential wrapper for message, so we can put it in collections *)
 Inductive exmsg : Type :=
-| Exm {A : Type} (msg : A) : exmsg.
+| Exm {A : Type} (msg : message A) : exmsg.
 
-Record channel_data := construct_channel
-  { properties : security_properties ;
-    type : channel_type ;
-    messages_sent : list (user_id * exmsg) ;
-    user_pointers : fmap user_id nat }.
-
-Definition channels := fmap channel_id channel_data.
-
-(* 
- *
- * The following are helper functions for permuting the universe when messages are published
- * or received.
- *
- *)
-Definition send_message u m ch_d :=
-  {| properties := ch_d.(properties) ;
-     type := ch_d.(type) ;
-     messages_sent := app ch_d.(messages_sent) [(u, m)] ;
-     user_pointers := ch_d.(user_pointers) |}.
-
-(* Helper function, finds first message sent by another user after last message seen if channel has 
-   been accessed before or from beginning if this is the user's first access. *)
-(* am I dealing with polymorphism right? does this pass in the "expected type" from the user cmd? *)
-Fixpoint recv_message' {A} ms (u : user_id) i : option A :=
-  match ms with
-  | [] => None
-  | (u', m) :: ms'
-    => match i with
-       | O => if u ==n u' then recv_message' ms' u O else Some m
-       | S n => recv_message' ms' u n                
-       end     
-  end.
-
-(* Get message from channel or else learn no valid message has been sent. *)
-Definition recv_message (ch_d : channel_data) (u : user_id) :=
-  match ch_d.(user_pointers) $? u with
-  | Some n => recv_message' ch_d.(messages_sent) u n
-  | None => recv_message' ch_d.(messages_sent) u O
-  end.
-
-(* Recorded in universe'; the next access by the user will not reconsume a previously seen
-   message. *)
-Definition inc_pointer ch_d u :=
-  match ch_d.(user_pointers) $? u with
-  | Some n => {| properties := ch_d.(properties) ;
-                 type := ch_d.(type) ;
-                 messages_sent := ch_d.(messages_sent) ;
-                 user_pointers := (ch_d.(user_pointers) $+ (u, S n)) |}
-  | None => {| properties := ch_d.(properties) ;
-               type := ch_d.(type) ;
-               messages_sent := ch_d.(messages_sent) ;
-               user_pointers := (ch_d.(user_pointers) $+ (u, 1)) |}
-  end.
-
-(*
- *
- * Properties of channels that allow reading or writing only under some circumstances.
- *
- *)
-Definition is_default_channel_owner user1 ch_ty :=
-  forall user2, ch_ty = Default user1 user2 \/ ch_ty = Default user2 user1.
-
-(* Deserving of its own definition because in broadcasts integrity <-> authenticity since we decided that 
-   giving a user "too much security" is better than making the sets of properties and channel types 
-   invalid. A "CIA Broadcast" channel is invalid. *)
-Definition I_A_IA_properties ps := ps = construct_properties false true true \/
-                                   ps = construct_properties false false true \/
-                                   ps = construct_properties false true false.
-
-Definition is_valid_IA_broadcast user ch_d :=
-  ch_d.(type) = Broadcast user /\ I_A_IA_properties ch_d.(properties).
-
-Definition is_C_broadcast ch_d :=
-  forall user, ch_d.(type) = Broadcast user /\ ch_d.(properties) = construct_properties true false false.
-
-Definition is_valid_C_broadcast user1 ch_d :=
-  forall user2, (ch_d.(type) = Default user1 user2 \/ ch_d.(type) = Default user2 user1) /\
-                ch_d.(properties) = construct_properties true false false.
-
-Definition is_IA_broadcast ch_d :=
-  forall user, ch_d.(type) = Broadcast user /\ I_A_IA_properties ch_d.(properties).
+Definition channels := fmap channel_id (set exmsg).
 
 Inductive cmd : Type -> Type :=
 | Return {result : Type} (r : result) : cmd result
 | Bind {result' result} (c1 : cmd result') (c2 : result' -> cmd result) : cmd result
-| Send {msg_ty : Type} (m : msg_ty) (ch_id : channel_id) : cmd unit
-| Recv {msg_ty : Type} (ch_id : channel_id) : cmd msg_ty
-| CreateChannel (p : security_properties) : cmd channel_id.
+| Send {msg_ty : Type} (m : message msg_ty) (ch_id : channel_id) : cmd unit
+| Recv {msg_ty : Type} (ch_id : channel_id) : cmd (message msg_ty)
+| CreateChannel : cmd channel_id.
 
 Notation "x <- c1 ; c2" := (Bind c1 (fun x => c2)) (right associativity, at level 75).
 
-Record universe (A : Type) : Type
-  := construct_universe
-       { channel_vector : fmap channel_id channel_data ;
-         users : user_list (cmd A)
-       }.
+Record user :=
+  { protocol : cmd unit ;
+    perms : permissions }.
 
-Inductive step_user : forall A, user_id * channels * cmd A -> user_id * channels * cmd A -> Prop :=
-| StepBindRecur : forall u result result' (c1 c1' : cmd result') (c2 : result' -> cmd result) cv cv',
-    step_user (u, cv, c1) (u, cv', c1') ->
-    step_user (u, cv, (Bind c1 c2)) (u, cv', (Bind c1' c2))
-| StepBindProceed : forall u (result result' : Type) (v : result') (c2 : result' -> cmd result) cv,
-    step_user (u, cv, (Bind (Return v) c2)) (u, cv, c2 v)
-| StepCreateChannel : forall u ch_id p cv,
+Record universe := construct_universe
+                     { channel_vector : fmap channel_id channels ;
+                       users : fmap user_id user}.
+
+(* write as inductive relation *)
+Fixpoint chs_search {A} (m : message A) : list (channel_id * permission) :=
+  match m with
+  | Permission id p => [(id, p)]
+  | Content _ => []
+  | MsgPair m1 m2 => chs_search m1 ++ chs_search m2        
+  end.
+
+Definition permission_subset p1 p2 : Prop :=
+  p1 = construct_permission true true \/
+  (p1 = construct_permission true false /\ p2.(write) = false) \/
+  (p1 = construct_permission false true /\ p2.(read) = false) \/
+  (p1 = construct_permission false false /\
+   p2 = construct_permission false false).
+
+Fixpoint msg_permissions_valid {A} (m : message A) ps : Prop :=
+  List.Forall
+    (fun '(id, ps_sent) =>
+      match ps $? id with
+      | Some p => permission_subset ps_sent p
+      | None => False
+      end)
+    (chs_search m).
+    
+
+Fixpoint add_chs_to_set (ks : list (channel_id * permission)) (ps : permissions) :=
+  match ks with
+  | [] => ps
+  | (id, perm) :: ks' => (add (add_chs_to_set ks' ps) id perm)
+  end.
+
+Inductive step_user : forall A, channels * cmd A * permissions -> channels * cmd A * permissions -> Prop :=
+| StepBindRecur : forall result result' (c1 c1' : cmd result') (c2 : result' -> cmd result) cv cv' ps ps',
+    step_user (cv, c1, ps) (cv', c1', ps') ->
+    step_user (cv, (Bind c1 c2), ps) (cv', (Bind c1' c2), ps')
+| StepBindProceed : forall (result result' : Set) (v : result') (c2 : result' -> cmd result) cv ps,
+    step_user (cv, (Bind (Return v) c2), ps) (cv, c2 v, ps)
+| StepCreateChannel : forall ch_id cv ps,
     ~(ch_id \in dom cv) ->
-    (* Unclear how to handle this for authenticity; it can work but only if there are two parties and 
-       there is no way of telling at this stage. *)
-    step_user (u, cv, (CreateChannel p))
-              (u, (cv $+ (ch_id, construct_channel p Symmetric [] $0)), (Return ch_id))
-| StepSendBroadcast : forall u cv (ch_id : channel_id) (ch_d : channel_data) {m_ty : Type} (m : m_ty),
+    step_user (cv, CreateChannel, ps)
+              (cv $+ (ch_id, {}), Return ch_id, ps $+ (ch_id, creator_permission))
+| StepSend : forall A cv (m : message A) ch_id ps ch_d b,
+    ps $? ch_id = Some {| read := b ; write := true |} ->
     cv $? ch_id = Some ch_d ->
-    (is_valid_IA_broadcast u ch_d \/ is_C_broadcast ch_d) ->
-    step_user (u, cv, (Send m ch_id))
-              (u, cv $+ (ch_id, send_message u (Exm m) ch_d), (Return tt))
-| StepSendSymmetric : forall u cv (ch_id : channel_id) {m_ty : Type} (m : m_ty) ch_d,
+    msg_permissions_valid m ps ->
+    step_user (cv, Send m ch_id, ps) (cv $+ (ch_id, {Exm m} \cup ch_d) , Return tt, ps)
+| StepRecv : forall A (cv cv' : channels) ch_d ps (m : message A) ch_id (ms ms' : list (user_id * exmsg)) b,
     cv $? ch_id = Some ch_d ->
-    ch_d.(type) = Symmetric ->
-    (* check user set of allowed channels for ch_id, check if CIA is valid *)
-    step_user (u, cv, Send m ch_id)
-              (u, cv $+ (ch_id, send_message u (Exm m) ch_d), Return tt)
-| StepSendDefault : forall u cv ch_d (ch_id : channel_id) {m_ty : Type} (m : m_ty),
-    cv $? ch_id = Some ch_d ->
-    is_default_channel_owner u ch_d.(type) ->
-    step_user (u, cv, Send m ch_id)
-              (u, cv $+ (ch_id, send_message u (Exm m) ch_d), Return tt)
-| StepRecvBroadcast : forall u cv ch_d (ch_id : channel_id) {msg_ty : Type} (m : msg_ty) ,
-    (* check if m is a symmetric channel id; add to set of allowed channels *)
-    cv $? ch_id = Some ch_d ->
-    (is_valid_C_broadcast u ch_d \/ is_IA_broadcast ch_d) ->
-    recv_message ch_d u = Some (Exm m) ->
-    step_user (u, cv, (Recv ch_id))
-              (u, cv $+ (ch_id, inc_pointer ch_d u), (Return m))
-| StepRecvSymmetric : forall u cv ch_d ch_id {m_ty : Type} (m : m_ty),
-    (* check set of allowed channels for ch_id *)
-    cv $? ch_id = Some ch_d ->
-    recv_message ch_d u = Some (Exm m) ->
-    (* check if m is a symmetric channel id; add to set of allowed channels *)
-    step_user (u, cv, (Recv ch_id))
-              (u, cv $+ (ch_id, inc_pointer ch_d u), (Return m))
-| StepRecvDefault : forall u cv ch_id ch_d {m_ty : Type} (m : m_ty),
-    cv $? ch_id = Some ch_d ->
-    is_default_channel_owner u ch_d.(type) ->
-    recv_message ch_d u = Some (Exm m) ->
-    (* check if m is a symmetric channel id; add to set of allowed channels *)
-    step_user (u, cv, Recv ch_id)
-              (u, cv $+ (ch_id, (inc_pointer ch_d u)), Return m).
-
-Inductive step_universe : forall {A : Type}, universe A -> universe A -> Prop :=
-| StepUser : forall A (U : universe A) u u_d cs' u_d',
-    In (u,u_d) U.(users) ->
-    (* U.(users) $? u = Some u_d -> *)
-    step_user (u, U.(channel_vector), u_d) (u, cs', u_d') ->
-    step_universe U (construct_universe cs' (updateUserList U.(users) u u_d')).
-
-Example ping : user_list (cmd nat) :=
-    (0, _ <- (Send 1 1) ; (Recv 1))
- :: (1, r <- (Recv 0) ; _ <- (Send 0 0) ; Return r)
- :: [].
-
-Example ping_universe :=
-{| channel_vector := $0 $+ (1, {| properties := {| confidentiality := true ;
-                                                   integrity := true ;
-                                                   authenticity := true |} ;
-                                  type := Default 1 2 ;
-                                  messages_sent := [] ;
-                                  user_pointers := $0 |}) ;
-   users := ping |}.
-
-Check ping_universe.
+    ps $? ch_id = Some {| read := true ; write := b |} ->
+    (Exm m) \in ch_d ->
+    step_user (cv, Recv ch_id, ps)
+              (cv, Return m, add_chs_to_set (chs_search m) ps).
